Proof optimization

Lambda.v
@@ -50,21 +50,42 @@ Fixpoint subst (t: Term) (a' a: Name) : Term :=
   | Lam (c,t) => Lam ((subst_name c a' a), (subst t a' a))
   end.
 
+Lemma subst_notin_atm t a b: b ∉ atm1 t → subst t a b = t.
+Proof. induction t; intros.
+  - simpl in *; unfold subst_name. admit.
+  - admit.
+  - admit.
+Admitted.   
+
 Inductive aeq: Term → Term → Prop :=
 | AeqVar: ∀ a, aeq (Var a) (Var a)
 | AeqApp: ∀ m n m' n', aeq m m' → aeq n n' → aeq (App m n) (App m' n')
-| AeqAbs: ∀ (a b c: Name) (m n: Term),
+| AeqAbs: ∀ (a b: Name) (m n: Term), ∀ c,
     (c <> a ∧ c <> b) → (c ∉ atm1 m ∧ c ∉ atm1 n) →
     aeq (subst m c a) (subst n c b) → aeq (Lam (a,m)) (Lam (b,n)).
 
 (* Necessario alguma relacao proper sobre os argumentos de aeq para
   facilitar reescrita *)
 
-Lemma aeq_subst: ∀ m n a b, aeq m n → aeq (subst m a b) (subst n a b).
-Proof. Admitted.
+Check not_eq_sym.
 
-#[export] Instance subst_proper: Proper (aeq ==> eq ==> eq ==> aeq) subst.
-Proof. repeat intro; subst; apply aeq_subst; auto. Qed.
+Lemma subst_equal: ∀ m a, (subst m a a) = m.
+Proof. 
+  induction m using term_ind_general; intros; simpl. 
+  - unfold subst_name; destruct (_ =n _); subst; constructor.
+  - rewrite IHm1, IHm2; reflexivity.
+  - unfold subst_name; destruct (_ =n _); subst.
+    + rewrite IHm; reflexivity.
+    + rewrite IHm; reflexivity.
+Qed.     
+
+Lemma aeq_subst: ∀ m n a c, 
+  c ≠ a → c ∉ atm1 m → c ∉ atm1 n →
+  aeq m n → aeq (subst m c a) (subst n c a).
+Proof. intros; induction H. Admitted.
+
+(* #[export] Instance subst_proper: Proper (aeq ==> eq ==> eq ==> aeq) subst.
+Proof. repeat intro; subst; apply aeq_subst; auto. Qed. *)
 
 #[export] Instance: Equiv Term := aeq.
 #[export] Instance: Reflexive aeq.
@@ -72,11 +93,11 @@ Proof.
   intro x; induction x using term_ind_general.
   - constructor.
   - constructor; auto.
-  - econstructor.
-    + (* facil, basta pegar um C diferente *) admit.
-    + (* facil, basta pegar um C diferente *) admit.
-    + apply aeq_subst; auto.
-Admitted.
+  - destruct (exist_fresh ({[a]} ∪ (atm1 x))) as [c Hc]; apply AeqAbs with (c := c).
+    + split; set_solver.
+    + split; set_solver. 
+    + apply aeq_subst; set_solver.
+Qed.
 
 #[export] Instance: Symmetric aeq.
 Proof.
@@ -164,67 +185,94 @@ Admitted.
 From Nominal Require Import Instances.SupportedFunctions
   Instances.Name Instances.Prod Instances.Perm.
 
-Lemma fun_eq `{Nominal X, Nominal Y} x y (f: X →ₛ Y): x ≡ y → f x ≡ f y.
-Proof. intros XY; rewrite XY; reflexivity. Qed.
-
 Definition FCB `{Nominal X, Nominal Y} (f: X →ₛ Y) :=
   { a | a ∉ (support f) ∧ (∀ x: X, a # (f x)) }.
- 
-Lemma perm_distr w z (p q: Perm): ⟨w,z⟩ • (p + q) ≡ (⟨w,z⟩ • p) + (⟨w,z⟩ • q).
-Proof. 
-  unfold action, perm_action; rewrite <-perm_inv, !grp_assoc. 
-  assert (HH: ⟨ w, z ⟩ + p + ⟨ w, z ⟩ + ⟨ w, z ⟩ + q + ⟨ w, z ⟩ ≡ ⟨ w, z ⟩ + p + (⟨ w, z ⟩ + ⟨ w, z ⟩) + q + ⟨ w, z ⟩).
-  { rewrite !grp_assoc; reflexivity. }
-  rewrite HH; clear HH.
-  rewrite perm_duplicate.
-  assert (HH: ⟨ w, z ⟩ + p + ɛ + q + ⟨ w, z ⟩ ≡ ⟨ w, z ⟩ + p + (ɛ + (q + ⟨ w, z ⟩))).
-  { rewrite !grp_assoc; reflexivity. } rewrite HH; clear HH.
-  rewrite grp_left_id, !grp_assoc; reflexivity.
-Qed.
 
-Lemma fun_1 `{Nominal X, Nominal Y} (p : Perm) (f: X →ₛ Y) (x : X):
-  p • (f x) ≡ (p • f)(p • x).
+(* Theorem freshness_theorem `{Nominal X} (f: Name →ₛ X): 
+  (∃ (c: Name), c ∉ support f ∧ c # (f c)) → 
+  ∀ a b, a # f → b # f → f a ≡ f b.
 Proof.
-  unfold action at 2; unfold fun_supp_act; simpl. 
-  rewrite perm_left_inv; reflexivity.
-Qed.
 
-Lemma name_action_left (a b: Name) : ⟨ a, b ⟩ • a ≡ b.
-Proof. unfold action, name_action; apply perm_swap_left. Qed.
+They are both provable
+*)
 
-Lemma name_action_right (a b: Name) : ⟨ a, b ⟩ • b ≡ a.
-Proof. unfold action, name_action; apply perm_swap_right. Qed.
-
-Theorem fresh_2 `{Nominal X} (f: Name →ₛ X): 
-  (∃ (a: Name), a ∉ support f ∧ a # (f a)) → 
-  ∀ b c, b # f ∧ c # f → f b ≡ f c.
+Theorem freshness_theorem `{Nominal X} (f: Name →ₛ X): 
+  ∀ a b, (∃ (c: Name), c ∉ support f ∧ c # (f c)) → 
+  a # f → b # f → f a ≡ f b.
 Proof. 
-  intros [a []] ? ? []. 
-  rewrite <-(fresh_fixpoint a b f) at 1; auto; try (apply support_fresh; assumption).
-  rewrite <-(fresh_fixpoint a c f) at 2; auto; try (apply support_fresh; assumption).
+  intros ? ? [c []] ? ?. 
+  rewrite <-(fresh_fixpoint c a f) at 1; auto; try (apply support_fresh; assumption).
+  rewrite <-(fresh_fixpoint c b f) at 2; auto; try (apply support_fresh; assumption).
   unfold action, fun_supp_act; simpl; rewrite <-!perm_inv, !name_action_right.
-  destruct (decide (a = b)), (decide (a = c)); subst.
-  - rewrite perm_action_equal; reflexivity.
-  - rewrite perm_action_equal; rewrite fresh_fixpoint.
-    + reflexivity.
-    + assumption.
-    + apply fresh_fun_supp; auto; apply name_neq_fresh_iff, not_eq_sym; assumption.
-  - rewrite perm_action_equal; rewrite fresh_fixpoint.
-    + reflexivity.
-    + assumption.
-    + apply fresh_fun_supp; auto; apply name_neq_fresh_iff, not_eq_sym; assumption.
-  - rewrite 2fresh_fixpoint; try reflexivity; try assumption;
+  destruct (decide (c = a)), (decide (c = b)); subst; try rewrite perm_action_equal.
+  - reflexivity.
+  - rewrite fresh_fixpoint; [reflexivity | assumption | idtac].
+    apply fresh_fun_supp; auto; apply name_neq_fresh_iff, not_eq_sym; assumption.
+  - rewrite fresh_fixpoint; [reflexivity | assumption | idtac].
+    apply fresh_fun_supp; auto; apply name_neq_fresh_iff, not_eq_sym; assumption.
+  - rewrite !fresh_fixpoint; try reflexivity; try assumption;
       apply fresh_fun_supp; auto; apply name_neq_fresh_iff, not_eq_sym; assumption.
 Qed.
 
-Lemma fresh_respectfull (A B: NameSet): A ≡ B → fresh A ≡ fresh B.
-Proof. intros AB; rewrite AB; reflexivity. Qed.
-
 From Nominal Require Import Alpha NameAbstraction.
+
+Lemma perm_distr_1 (a b w z: Name) (p: Perm):
+  w ≠ a → w ≠ b → z ≠ a → z ≠ b →
+  ⟨a,b⟩ + (⟨w, z⟩•p) ≡ (⟨w, z⟩•⟨a,b⟩) + (⟨w,z⟩•p).
+Proof.
+  intros; rewrite <-(fresh_fixpoint w z (⟨ a, b ⟩)) at 1; auto;
+  apply support_fresh; set_solver.
+Qed.
+
+Lemma perm_distr_2 (a b w z: Name) (p: Perm):
+  (⟨w,z⟩•⟨a,b⟩) + (⟨w,z⟩•p) ≡ ⟨w,z⟩•(⟨a,b⟩ + p).
+Proof.
+  unfold action, perm_action; rewrite <-perm_inv, !grp_assoc.
+  assert (H: ⟨w,z⟩+⟨a,b⟩+⟨w,z⟩+⟨w,z⟩+p+⟨w,z⟩ ≡ ⟨w,z⟩+⟨a,b⟩+(⟨w,z⟩+⟨w,z⟩)+p+⟨w,z⟩). {
+    rewrite !grp_assoc; reflexivity.
+  }
+  rewrite H, perm_duplicate; clear H.
+  assert (H: ⟨w,z⟩+⟨a,b⟩+ɛ+p+⟨w,z⟩ ≡ ⟨w,z⟩+⟨a,b⟩+(ɛ+(p+⟨w,z⟩))). {
+    rewrite !grp_assoc; reflexivity.
+  }
+  rewrite H, grp_left_id, !grp_assoc; reflexivity.
+Qed.
+
+Lemma perm_distr_3 (a b w z: Name) (p: Perm):
+  w ∉ perm_dom p → z ∉ perm_dom p → w ≠ a → z ≠ a →
+  ⟨w,z⟩•⟨a,b⟩+p ≡ ⟨a,⟨w,z⟩•b⟩+p.
+Proof.
+  intros Pw Pz ? ?; rewrite perm_distr; do 2 unfold action at 1; unfold perm_action.
+  assert (HH1: -⟨w,z⟩+(⟨a,b⟩+⟨w,z⟩)+(-⟨w,z⟩+(p+⟨w,z⟩)) ≡ (⟨a,⟨w,z⟩•b⟩+p)). {
+    rewrite <-perm_inv, !grp_assoc.
+    assert (HH2: ⟨w,z⟩+⟨a,b⟩+⟨w,z⟩+⟨w,z⟩+p+⟨w,z⟩ ≡ ⟨w,z⟩+⟨a,b⟩+p+⟨w,z⟩). {
+      assert (HH3: ⟨w,z⟩+⟨a,b⟩+⟨w,z⟩+⟨w,z⟩+p+⟨w,z⟩ ≡ ⟨w,z⟩+⟨a,b⟩+(⟨w,z⟩+⟨w,z⟩)+p+⟨w,z⟩). {
+      rewrite !grp_assoc; reflexivity.
+      } rewrite HH3, perm_duplicate; clear HH3.
+      assert (HH3: ⟨w,z⟩+⟨a,b⟩+ɛ+p+⟨w,z⟩ ≡ ⟨w,z⟩+⟨a,b⟩+(ɛ+(p+⟨w,z⟩))). {
+        rewrite !grp_assoc; reflexivity.
+      } rewrite HH3, grp_left_id, !grp_assoc; reflexivity.
+    } rewrite HH2; clear HH2; pose proof (perm_notin_dom_comm w z p Pw Pz) as HH.
+    assert (HH2: ⟨w,z⟩+⟨a,b⟩+p+⟨w,z⟩ ≡ ⟨w,z⟩+⟨a,b⟩+⟨w,z⟩+p). {
+      assert (HH3: ⟨w,z⟩+⟨a,b⟩+p+⟨w,z⟩ ≡ ⟨w,z⟩+⟨a,b⟩+(p+⟨w,z⟩)). {
+        rewrite !grp_assoc; reflexivity.
+      } rewrite HH3, <-HH, grp_assoc; reflexivity.
+    } rewrite HH2; clear HH2.
+    pose proof (perm_comm_distr a b ⟨ w, z ⟩) as H2; rewrite perm_swap_neither in H2;
+    try (apply not_eq_sym; auto).
+    assert (HH2: ⟨w,z⟩+⟨a,b⟩+⟨w,z⟩+p ≡ ⟨w,z⟩+(⟨a,b⟩+⟨w,z⟩)+p). {
+      rewrite !grp_assoc; reflexivity.
+    } rewrite HH2, H2, !grp_assoc, perm_duplicate, grp_left_id; 
+    unfold action; simpl; reflexivity.
+  }
+  assert (HH2: (-⟨w,z⟩+(⟨a,b⟩+⟨w,z⟩)+(-⟨w,z⟩+(p+⟨w,z⟩))) ≡ (⟨a,⟨w,z⟩•b⟩+p)). {
+    rewrite HH1; reflexivity.
+  } rewrite HH2; reflexivity.
+Qed.
 
 Definition perm_rect_iterator_supported_abstraction `{Nominal X}
   (A: NameSet)
-  (fvar : Name →ₛ X) (* support fvar ⊂ A *)
+  (fvar : Name →ₛ X)
   (fapp : (X * X) →ₛ X)
   (flam : [𝔸]X →ₛ X) 
   {lamFCB : FCB flam} : Term → (Perm →ₛ X).
@@ -243,184 +291,79 @@ Proof.
       end
   ).
   all: swap 5 6.
-  - repeat intro; rewrite H1; reflexivity.
-  - abstract (intros w z []%not_elem_of_union []%not_elem_of_union p; 
+  - intros ? ? HH; rewrite HH; reflexivity.
+  - intros w z []%not_elem_of_union []%not_elem_of_union p; 
     unfold action at 3; unfold perm_action;
     rewrite <-2!gact_compat, <-perm_inv, (fresh_fixpoint _ _ a);
       try (apply support_fresh; assumption);
       rewrite perm_inv at 2; rewrite <-fsupp_action, fresh_fixpoint;
-        try (apply support_fresh; assumption); reflexivity).
-  - repeat intro; rewrite H1; reflexivity.
+        try (apply support_fresh; assumption); reflexivity.
+  - intros ? ? HH; rewrite HH; reflexivity.
   - intros w z [[]%not_elem_of_union ?]%not_elem_of_union [[]%not_elem_of_union ?]%not_elem_of_union p.
     rewrite <-(fresh_fixpoint w z (F m)) at 1; try (apply support_fresh; assumption).
     rewrite <-(fresh_fixpoint w z (F n)) at 1; try (apply support_fresh; assumption).
-    rewrite <-2!fun_1, <-prod_act; rewrite perm_inv at 2; rewrite <-fsupp_action.
+    rewrite <-2!fun_equivar, <-prod_act; rewrite perm_inv at 2; rewrite <-fsupp_action.
     rewrite fresh_fixpoint; try (apply support_fresh; assumption); reflexivity.
   - intros w z Hw Hz p; cbn zeta.
     set (g := (λₛ⟦ support flam ∪ support (F m) ∪ support a ∪ support (⟨ w, z ⟩ • p) ∪ A ⟧ a' : Name, flam [a'](F m (⟨ a, a' ⟩ + (⟨ w, z ⟩ • p))))).
     set (h := (λₛ⟦ support flam ∪ support (F m) ∪ support a ∪ support p ∪ A ⟧ a' : Name, flam [a'](F m (⟨ a, a' ⟩ + p)))).
     destruct (exist_fresh (support flam ∪ support (F m) ∪ support a ∪ support w ∪ support z ∪ support (⟨ w, z ⟩ • p) ∪ support p ∪ A)) as [b Hb].
-    assert (HH1: (∃ (b: Name), b ∉ (support flam ∪ support (F m) ∪ support a ∪ support (⟨ w, z ⟩ • p) ∪ A) ∧ b # (g b))). {
-       exists b; split.
-       - set_solver.
-       - subst g; simpl; destruct lamFCB as [c [Hc1 Hc2]].
-         specialize (Hc2 [c](⟨ c, b ⟩ • (F m (⟨ a, b ⟩ + (⟨ w, z ⟩ • p))))).
+    rewrite (freshness_theorem g (fresh (support g)) b), (freshness_theorem h (fresh (support h)) b);
+    try (apply fresh_support_fresh); try (apply support_fresh; subst h g; unfold support at 1; simpl; set_solver).
+    all: swap 1 2. all: swap 2 3.
+    + exists b; split.
+      * set_solver.
+      * subst h; simpl; destruct lamFCB as [c [? Hc2]].
+         specialize (Hc2 [c](⟨ c, b ⟩ • (F m (⟨ a, b ⟩ + p)))).
          apply ((fresh_equivariant ⟨c,b⟩ _ _)) in Hc2; rewrite perm_swap_left in Hc2.
-         assert (HH: (⟨ c, b ⟩•(flam [c](⟨ c, b ⟩ • F m (⟨ a, b ⟩ + (⟨ w, z ⟩ • p))))) ≡ flam [b](F m (⟨a,b⟩ + (⟨ w, z ⟩ • p)))).
-         { rewrite fun_1, nabs_action, name_action_left, (fresh_fixpoint _ _ flam).
-            + apply fun_eq, nabs_inv, perm_action_duplicate. 
-            + apply support_fresh; assumption.
-            + apply support_fresh; set_solver.
-         }
-         rewrite <-HH; apply Hc2.
-    }
-    assert (HH2: (∃ (b: Name), b ∉ (support flam ∪ support (F m) ∪ support a ∪ support p ∪ A) ∧ b # (h b))). { 
-      exists b; split.
-      - set_solver.  
-      - subst h; simpl; destruct lamFCB as [c [Hc1 Hc2]].
-        specialize (Hc2 [c](⟨ c, b ⟩ • (F m (⟨ a, b ⟩ + p)))).
+         rewrite <-(fresh_fixpoint c b flam), fsupp_action, <-perm_inv, nabs_action, name_action_right;
+         [apply Hc2 | |]; apply support_fresh; set_solver.
+    + exists b; split.
+      * set_solver.
+      * subst g; simpl; destruct lamFCB as [c [? Hc2]].
+        specialize (Hc2 [c](⟨ c, b ⟩ • (F m (⟨ a, b ⟩ + (⟨ w, z ⟩ • p))))).
         apply ((fresh_equivariant ⟨c,b⟩ _ _)) in Hc2; rewrite perm_swap_left in Hc2.
-        assert (HH: (⟨ c, b ⟩ • flam [c](⟨ c, b ⟩ • F m (⟨ a, b ⟩ + p))) ≡ flam [b](F m (⟨ a, b ⟩ + p))). {
-          rewrite fun_1, nabs_action, name_action_left, (fresh_fixpoint _ _ flam).
-          + apply fun_eq, nabs_inv, perm_action_duplicate.
-          + apply support_fresh; assumption.
-          + apply support_fresh; set_solver.  
-        }
-        rewrite <-HH; apply Hc2.
-    }
-    pose proof fresh_2 as F1; pose proof fresh_2 as F2.
-    specialize (F1 g HH1 (fresh (support g)) b). specialize (F2 h HH2 (fresh (support h)) b).
-    rewrite F1; try (split; [apply fresh_support_fresh | apply support_fresh; subst g; unfold support at 1; simpl; set_solver]).
-    rewrite F2; try (split; [apply fresh_support_fresh | apply support_fresh; subst h; unfold support at 1; simpl; set_solver]). 
-    subst g h; simpl.
-    clear HH1 HH2 F1 F2.
-    assert (HH1: (⟨a,b⟩ + (⟨w, z⟩•p)) ≡ (⟨w, z⟩•⟨a,b⟩) + (⟨w,z⟩•p)). {
-      rewrite <-(fresh_fixpoint w z (⟨ a, b ⟩)) at 1. reflexivity.
-      - apply support_fresh; unfold support; simpl; apply not_elem_of_union; split.
-        + apply not_elem_of_union; split; unfold support,name_support in *; simpl in *;
-          set_solver.
-        + set_solver.
-      - apply support_fresh; unfold support; simpl; apply not_elem_of_union; split.
-        + apply not_elem_of_union; split; unfold support,name_support in *; simpl in *;
-          set_solver.
-        + set_solver.   
-    }
-    assert (HH2: (⟨w,z⟩•⟨a,b⟩) + (⟨w,z⟩•p) ≡ ⟨w,z⟩•(⟨a,b⟩ + p)). {
-      unfold action, perm_action; rewrite <-perm_inv, !grp_assoc.
-      assert (HHH2: ⟨ w, z ⟩ + ⟨ a, b ⟩ + ⟨ w, z ⟩ + ⟨ w, z ⟩ + p + ⟨ w, z ⟩ ≡ ⟨ w, z ⟩ + ⟨ a, b ⟩ + (⟨ w, z ⟩ + ⟨ w, z ⟩) + p + ⟨ w, z ⟩). {
-        rewrite !grp_assoc; reflexivity.
-      }
-      rewrite HHH2, perm_duplicate.
-      assert (HHH3: ⟨ w, z ⟩ + ⟨ a, b ⟩ + ɛ + p + ⟨ w, z ⟩ ≡ ⟨ w, z ⟩ + ⟨ a, b ⟩ + (ɛ + (p + ⟨ w, z ⟩))). {
-        rewrite !grp_assoc; reflexivity.
-      }
-      rewrite HHH3, grp_left_id, !grp_assoc; reflexivity.
-    }
-    assert (HH: flam [b](F m (⟨ a, b ⟩ + (⟨ w, z ⟩ • p))) ≡ flam [b]((⟨ w, z ⟩ • F m) (⟨ w, z ⟩ • ⟨ a, b ⟩ + p))). {
-      apply fun_eq, nabs_inv; 
-      rewrite HH1, HH2.
-      rewrite <-(fresh_fixpoint w z (F m)) at 1; try (apply support_fresh; set_solver).
+        rewrite <-(fresh_fixpoint c b flam), fsupp_action, <-perm_inv, nabs_action, name_action_right;
+        [apply Hc2 | |]; apply support_fresh; set_solver.
+    + subst g h; simpl.
+      assert (HH: flam [b](F m (⟨a,b⟩+(⟨w,z⟩•p))) ≡ flam [b]((⟨w,z⟩•(F m)) (⟨w,z⟩•⟨a,b⟩+p))). {
+      apply fsupp_equiv, nabs_inv. 
+      rewrite perm_distr_1, perm_distr,<-(fresh_fixpoint w z (F m)) at 1;
+      try reflexivity; try (apply support_fresh); set_solver.
+      } rewrite HH; clear HH.
+      rewrite <-(fresh_fixpoint w z b) at 1; try (apply support_fresh; set_solver).
+      assert (HH: flam [⟨w,z⟩•b]((⟨w,z⟩•(F m)) (⟨w,z⟩•⟨a,b⟩+p)) ≡ flam ([⟨w,z⟩•b](⟨w,z⟩•(F m (⟨a,b⟩+p))))). {
+      apply fsupp_equiv, nabs_inv. rewrite fun_equivar; reflexivity.
+      } rewrite HH; clear HH.
+      rewrite <-nabs_action,<-fsupp_action, fresh_fixpoint; try (apply support_fresh; set_solver).
       reflexivity.
-    }
-    rewrite HH; clear HH1 HH2 HH.
-    assert (HH: flam [b]((⟨ w, z ⟩ • F m) (⟨ w, z ⟩ • ⟨ a, b ⟩ + p)) ≡ flam [⟨ w, z ⟩ •b]((⟨ w, z ⟩ • F m) (⟨ w, z ⟩ • ⟨ a, b ⟩ + p))). {
-      apply fun_eq. rewrite <-(fresh_fixpoint w z b) at 1; try (apply support_fresh; set_solver).
-      reflexivity.
-    }
-    rewrite HH; clear HH.
-    assert (HH: flam [⟨ w, z ⟩•b]((⟨ w, z ⟩ • F m) (⟨ w, z ⟩ • ⟨ a, b ⟩ + p)) ≡ flam ([⟨ w, z ⟩•b](⟨ w, z ⟩•(F m (⟨a, b ⟩ + p))))). {
-      apply fun_eq, nabs_inv. rewrite fun_1. reflexivity.
-    }
-    rewrite HH; clear HH.
-    assert (HH: flam [⟨ w, z ⟩ • b](⟨ w, z ⟩ • F m (⟨ a, b ⟩ + p)) ≡ flam (⟨ w, z ⟩•([b](F m (⟨ a, b ⟩ + p))))). {
-      apply fun_eq; rewrite nabs_action; reflexivity.
-    }
-    rewrite HH; clear HH.
-    rewrite <-fsupp_action, fresh_fixpoint; try (apply support_fresh; set_solver).
-    reflexivity.
 Unshelve.
   (* show that h is supported *)
   intros w z Hw Hz b.
-  set (T := ⟨ w, z ⟩ • flam [⟨ w, z ⟩ • b](F m (⟨ a, ⟨ w, z ⟩ • b ⟩ + p))).
-  rewrite <-(fresh_fixpoint w z flam); try (apply support_fresh; set_solver).
-  rewrite fsupp_action, <-perm_inv, nabs_action.
-  assert (HH: flam [⟨ w, z ⟩ • b](⟨ w, z ⟩ • F m (⟨ a, b ⟩ + p)) ≡ flam [⟨ w, z ⟩ • b]((⟨ w, z ⟩ • F m) (⟨ w, z ⟩ • ⟨ a, b ⟩ + p))). {
-    apply fun_eq, nabs_inv; rewrite (fun_1 (⟨w,z⟩) (F m)). reflexivity.
-  }
-  rewrite HH; clear HH.
-  assert (HH: flam [⟨ w, z ⟩ • b]((⟨ w, z ⟩ • F m) (⟨ w, z ⟩ • ⟨ a, b ⟩ + p)) ≡ flam [⟨ w, z ⟩ • b]((F m (⟨ w, z ⟩ • ⟨ a, b ⟩ + p)))). {  
-    apply fun_eq, nabs_inv; rewrite (fresh_fixpoint w z (F m)); try (apply support_fresh; set_solver); reflexivity.
-  }
-  rewrite HH; clear HH.
-  assert (HH: flam [⟨ w, z ⟩ • b](F m (⟨ w, z ⟩ • ⟨ a, b ⟩ + p)) ≡ flam [⟨ w, z ⟩ • b](F m (⟨ a, ⟨ w, z ⟩ • b ⟩ + p))). {
-    apply fun_eq, nabs_inv.
-    rewrite perm_distr; unfold action at 1; unfold action at 1; unfold perm_action.
-    assert (HH: - ⟨ w, z ⟩ + (⟨ a, b ⟩ + ⟨ w, z ⟩) + (- ⟨ w, z ⟩ + (p + ⟨ w, z ⟩)) ≡ (⟨ a, ⟨ w, z ⟩ • b ⟩ + p)). {
-      rewrite <-perm_inv, !grp_assoc.
-      assert (HH1: ⟨ w, z ⟩ + ⟨ a, b ⟩ + ⟨ w, z ⟩ + ⟨ w, z ⟩ + p + ⟨ w, z ⟩ ≡ ⟨ w, z ⟩ + ⟨ a, b ⟩ + p + ⟨ w, z ⟩). {
-         assert (HHH: ⟨ w, z ⟩ + ⟨ a, b ⟩ + ⟨ w, z ⟩ + ⟨ w, z ⟩ + p + ⟨ w, z ⟩ ≡ ⟨ w, z ⟩ + ⟨ a, b ⟩ + (⟨ w, z ⟩ + ⟨ w, z ⟩) + p + ⟨ w, z ⟩). {
-         rewrite !grp_assoc; reflexivity. }
-         rewrite HHH, perm_duplicate.
-         assert (HHH1: ⟨ w, z ⟩ + ⟨ a, b ⟩ + ɛ + p + ⟨ w, z ⟩ ≡ ⟨ w, z ⟩ + ⟨ a, b ⟩ + (ɛ + (p + ⟨ w, z ⟩))). {
-          rewrite !grp_assoc; reflexivity.
-         } rewrite HHH1, grp_left_id, !grp_assoc; reflexivity.
-    }
-    rewrite HH1; pose proof (perm_notin_dom_comm w z p) as H1.
-    assert (HH2: ⟨ w, z ⟩ + ⟨ a, b ⟩ + p + ⟨ w, z ⟩ ≡ ⟨ w, z ⟩ + ⟨ a, b ⟩ + ⟨ w, z ⟩ + p). {
-      assert (HHH: ⟨ w, z ⟩ + ⟨ a, b ⟩ + p + ⟨ w, z ⟩ ≡ ⟨ w, z ⟩ + ⟨ a, b ⟩ + (p + ⟨ w, z ⟩)). {
-        rewrite !grp_assoc; reflexivity.
-      } rewrite HHH, <-H1; unfold support in *; set_solver.
-    }
-    rewrite HH2.
-    pose proof (perm_comm_distr a b ⟨ w, z ⟩); rewrite perm_swap_neither in H2;
-      try (apply not_eq_sym, name_neq_fresh_iff, support_fresh; set_solver).
-    assert (HH3: ⟨ w, z ⟩ + ⟨ a, b ⟩ + ⟨ w, z ⟩ + p ≡ ⟨ w, z ⟩ + (⟨ a, b ⟩ + ⟨ w, z ⟩) + p). {
-      rewrite !grp_assoc; reflexivity.
-    }
-    rewrite HH3, H2, !grp_assoc, perm_duplicate, grp_left_id; unfold action. simpl; reflexivity.
-  }
-  assert (HH1: F m (- ⟨ w, z ⟩ + (⟨ a, b ⟩ + ⟨ w, z ⟩) + (- ⟨ w, z ⟩ + (p + ⟨ w, z ⟩))) ≡ F m (⟨ a, ⟨ w, z ⟩ • b ⟩ + p)). {
-    rewrite HH; reflexivity.
-  }
-  rewrite HH1; reflexivity.
-  }
-  rewrite HH; subst T; reflexivity.
-- repeat intro; cbn zeta. set (a' := fresh _); set (b' := fresh _).
-  destruct (exist_fresh (support flam ∪ support (F m) ∪ support a ∪ support x ∪ support y ∪ support a' ∪ support b' ∪ A)) as [c Hc].
-  rewrite fresh_2 with (c := c), fresh_2 with (b := b') (c := c).
-  + simpl; apply fun_eq, nabs_inv, fun_eq, grp_op_proper; auto.
+  rewrite <-(fresh_fixpoint w z flam) at 2; try (apply support_fresh; set_solver).
+  rewrite fsupp_action, <-perm_inv, nabs_action; apply gact_proper, fsupp_equiv; auto.
+  rewrite (fun_equivar (⟨w,z⟩) (F m)), (fresh_fixpoint w z (F m)); try (apply support_fresh; set_solver).
+  rewrite perm_distr_3; set_solver.
+- intros x y Hxy; cbn zeta; set (a' := fresh _); set (b' := fresh _).
+  set (g := (λₛ⟦ _ ⟧ _ : Name, flam [_](F m (⟨ a, _ ⟩ + x)))).
+  set (h := (λₛ⟦ _ ⟧ _' : Name, flam [_](F m (⟨ a, _ ⟩ + y)))).
+  destruct (exist_fresh (support flam ∪ support (F m) ∪ support a ∪ support x ∪ support y ∪ support a' ∪ support b' ∪ A)) as [c Hc];
+  repeat (apply not_elem_of_union in Hc as [Hc ?]);
+  rewrite (freshness_theorem g a' c), (freshness_theorem h b' c);
+  try (apply fresh_support_fresh); try (apply support_fresh; subst h g; unfold support at 1; simpl; set_solver).
+  + simpl; apply fsupp_equiv, nabs_inv, fsupp_equiv, grp_op_proper; auto.
   + exists c; split.
-    * unfold support in *; subst a' b'; simpl in *; set_solver.
-    * simpl; destruct lamFCB as [d [Hd1 Hd2]].
-      specialize (Hd2 [d](⟨ d, c ⟩ • (F m (⟨ a, c ⟩ + y)))).
-      apply ((fresh_equivariant ⟨d,c⟩ _ _)) in Hd2; rewrite perm_swap_left in Hd2.
-      assert (HH: (⟨ d, c ⟩ • flam [d](⟨ d, c ⟩ • F m (⟨ a, c ⟩ + y))) ≡ flam [c](F m (⟨ a, c ⟩ + y))). {
-        rewrite fun_1, nabs_action, name_action_left, (fresh_fixpoint _ _ flam).
-        + apply fun_eq; unfold equiv, name_abstraction_equiv; apply alpha_inv_iff; left;
-          split; auto. rewrite perm_action_duplicate; reflexivity.
-        + apply support_fresh; assumption.
-        + repeat apply not_elem_of_union in Hc as [Hc ?]; apply support_fresh; assumption.
-      }
-      rewrite <-HH; apply Hd2.
-  + split; apply support_fresh; subst b'; unfold support in *; simpl in *.
-    * apply is_fresh.
-    * set_solver.  
+    * set_solver.
+    * subst h; simpl; destruct lamFCB as [d [? Hd]].
+       specialize (Hd [d](⟨d,c⟩•(F m (⟨a,c⟩ + y)))).
+       apply ((fresh_equivariant ⟨d,c⟩ _ _)) in Hd; rewrite perm_swap_left in Hd.
+       rewrite <-(fresh_fixpoint d c flam), fsupp_action, <-perm_inv, nabs_action, name_action_right;
+       [apply Hd | |]; apply support_fresh; set_solver.
   + exists c; split.
-    * unfold support in *; subst a' b'; simpl in *; set_solver.
-    * simpl. destruct lamFCB as [d [Hd1 Hd2]].
-      specialize (Hd2 [d](⟨ d, c ⟩ • (F m (⟨ a, c ⟩ + x)))).
-      apply ((fresh_equivariant ⟨d,c⟩ _ _)) in Hd2; rewrite perm_swap_left in Hd2.
-      assert (HH: (⟨ d, c ⟩ • flam [d](⟨ d, c ⟩ • F m (⟨ a, c ⟩ + x))) ≡ flam [c](F m (⟨ a, c ⟩ + x))). {
-        rewrite fun_1, nabs_action, name_action_left, (fresh_fixpoint _ _ flam).
-        + apply fun_eq; unfold equiv, name_abstraction_equiv; apply alpha_inv_iff; left;
-          split; auto. rewrite perm_action_duplicate; reflexivity.
-        + apply support_fresh; assumption.
-        + repeat apply not_elem_of_union in Hc as [Hc ?]; apply support_fresh; assumption.
-      }
-      rewrite <-HH; apply Hd2.
-  + split; apply support_fresh; subst a'; unfold support in *; simpl in *.
-  * apply is_fresh.
-  * set_solver.  
+  * set_solver.
+  * subst h; simpl; destruct lamFCB as [d [? Hd]].
+     specialize (Hd [d](⟨d,c⟩•(F m (⟨a,c⟩ + x)))).
+     apply ((fresh_equivariant ⟨d,c⟩ _ _)) in Hd; rewrite perm_swap_left in Hd.
+     rewrite <-(fresh_fixpoint d c flam), fsupp_action, <-perm_inv, nabs_action, name_action_right;
+     [apply Hd | |]; apply support_fresh; set_solver.
 Qed.
-
-Print perm_rect_iterator_supported_abstraction.
